proof/proof/advrpc.v
@@ -5,6 +5,19 @@ From New.proof.github_com.sanjit_bhat.pav Require Import
   safemarshal netffi.
 
 Module advrpc.
+
+Section defs.
+Context `{hG: heapGS Σ, !ffi_semantics _ _}.
+Context {sem : go.Semantics}.
+Collection W := sem.
+#[local] Set Default Proof Using "W".
+
+Definition is_Server (s : loc) : iProp Σ. Admitted.
+
+#[global] Instance is_Server_pers s : Persistent (is_Server s). Admitted.
+
+End defs.
+
 Section proof.
 Context `{hG: heapGS Σ, !ffi_semantics _ _}.
 Context {sem : go.Semantics} {package_sem : advrpc.Assumptions}.
@@ -13,6 +26,15 @@ Collection W := sem + package_sem.
 
 #[global] Instance : IsPkgInit (iProp Σ) advrpc := define_is_pkg_init True%I.
 #[global] Instance : GetIsPkgInitWf (iProp Σ) advrpc := build_get_is_pkg_init_wf.
+
+Lemma wp_Server_Serve s (addr : w64) :
+  {{{
+    is_pkg_init advrpc ∗
+    "#His_serv" ∷ is_Server s
+  }}}
+  s @! (go.PointerType advrpc.Server) @! "Serve" #addr
+  {{{ RET #(); True }}}.
+Proof. Admitted.
 
 End proof.
 End advrpc.
