proof/proof/alicebob.v
@@ -4,7 +4,7 @@ From New.proof.github_com.sanjit_bhat.pav Require Import prelude.
 From New.proof Require Import bytes time.
 From New.proof.github_com.goose_lang Require Import primitive std.
 From New.proof.github_com.sanjit_bhat.pav Require Import
-  auditor client cryptoffi ktcore server.
+  advrpc auditor client cryptoffi ktcore server.
 
 Module alicebob.
 
@@ -27,9 +27,8 @@ Collection W := sem + package_sem.
 #[global] Instance : IsPkgInit (iProp Σ) alicebob := define_is_pkg_init True%I.
 #[global] Instance : GetIsPkgInitWf (iProp Σ) alicebob := build_get_is_pkg_init_wf.
 
-(* [alice_leak] is whether alice's uid is adversarially controlled. *)
 Lemma wp_testAliceBob (serv_trust adtr_trust : Trust.t)
-    (alice_leak bob_leak : bool)
+    (alice_good bob_good : bool)
     (servAddr : w64) (servGood : bool) sl_adtrAddrs (adtrAddrs : list w64) :
   {{{
     is_pkg_init alicebob ∗
@@ -41,7 +40,33 @@ Lemma wp_testAliceBob (serv_trust adtr_trust : Trust.t)
   }}}
   @! alicebob.testAliceBob #servAddr #servGood #sl_adtrAddrs
   {{{ RET #(); True }}}.
-Proof. Admitted.
+Proof.
+  wp_start as "@". wp_auto.
+  iMod (mono_list_own_alloc ([] : list (nat * list w8))) as (alice_uidγ) "[Halice_puts _]".
+  iMod (mono_list_own_alloc ([] : list (nat * list w8))) as (bob_uidγ) "[Hbob_puts _]".
+  iAssert (
+    |={⊤}=>
+    match alice_good with
+    | true => mono_list_auth_own alice_uidγ 1 ([] : list (nat * list w8))
+    | false => client.ver.is_uid_inv alice_uidγ
+    end)%I with "[Halice_puts]" as "> Halice_good".
+  { case_match; [by iFrame|].
+    iApply inv_alloc.
+    iFrame. }
+  iAssert (
+    |={⊤}=>
+    match bob_good with
+    | true => mono_list_auth_own bob_uidγ 1 ([] : list (nat * list w8))
+    | false => client.ver.is_uid_inv bob_uidγ
+    end)%I with "[Hbob_puts]" as "> Hbob_good".
+  { case_match; [by iFrame|].
+    iApply inv_alloc.
+    iFrame. }
+  set ({[W64 0:=alice_uidγ; W64 1:=bob_uidγ]} : gmap w64 gname) as uidγs.
+  wp_apply (server.wp_New uidγs) as "* @".
+  wp_apply (server.wp_NewRpcServer with "[$Hlocks]") as "* @".
+  wp_apply advrpc.wp_Server_Serve.
+Admitted.
 
 End proof.
 End alicebob.
